

HW 2 :

①

a.) $x[n] = e^{jn\pi/6}$

$$x_{cs}[n] = \frac{1}{2} (x[n] + x^*[n])$$

$$x_{ca}[n] = \frac{1}{2} (x[n] - x^*[n])$$

$$x[n] = e^{jn\pi/6} \quad x^*[-n] = e^{jn\pi/6}$$

$$x_{cs}[n] = \frac{1}{2} (e^{jn\pi/6} + e^{jn\pi/6}) = \underline{e^{jn\pi/6}}$$

$$x_{ca}[n] = \frac{1}{2} (e^{jn\pi/6} - e^{jn\pi/6}) = \underline{0}$$

b.) $y[n] = -je^{-jn\pi/2}$ $y^*[n] = je^{-jn\pi/2}$

$$y_{cs}[n] = \frac{1}{2} (-je^{-jn\pi/2} + je^{-jn\pi/2}) = \underline{0}$$

$$y_{ca}[n] = \frac{1}{2} (-je^{-jn\pi/2} - je^{-jn\pi/2}) = \underline{-je^{-jn\pi/2}}$$

② Z-transform for $x[n] = \begin{Bmatrix} -1 & 0 & 1 & 2 & 3 & 4 \\ -2 & 5 & 1 & -3 & 5 & 3 \end{Bmatrix}$, $-1 \leq n \leq 4$
and $g[n] = x[n-3]$

$$Z\{x[n]\} = 3z^{-4} + 5z^{-3} - 3z^{-2} + z^{-1} + 5 - 2z = X(z)$$

$$Z\{g[n]\} \stackrel{\leftarrow 2 \leq n \leq 7}{=} 3z^{-7} + 5z^{-6} - 3z^{-5} + z^{-4} + 5z^{-3} - 2z^{-2} = G(z)$$

③

$$x[n] = \{2, -4, 1, -4\} \quad 1 \leq n \leq 4, \quad x[n] = 0 \text{ for all other } n$$

$$\mathcal{L}_1\{x[n]\} = \|x[n]\|_1 = \sum_{n=-1}^4 (|x[n]|)$$

$$= 2 + 4 + 1 + 4 = \boxed{\mathcal{L}_1 = 11}$$

$$\|x\|_p = \left(\sum_{n=-\infty}^{\infty} |x[n]|^p \right)^{1/p}$$

$$\|x\|_{\infty} = |x|_{\max}$$

$$\mathcal{L}_2\{x[n]\} = \|x[n]\|_2 = \sum_{n=-1}^4 (|x[n]|^2)^{1/2}$$

$$= \sqrt{2^2 + 4^2 + 1^2 + 4^2} = \sqrt{37} \Rightarrow \boxed{\mathcal{L}_2 = \sqrt{37}}$$

$$\mathcal{L}_{\infty}\{x[n]\} = |x|_{\max} = 4 \quad \boxed{\mathcal{L}_{\infty} = 4}$$